Interop: Example of TCB disentanglement for memcpy

src/arch/x64/interop/Memcpy.fst
@@ -18,6 +18,11 @@ open X64.Vale.State_i
 open X64.Vale.Decls_i
 open BufferViewHelpers
 open Interop_assumptions
+open X64.Vale.StateLemmas_i
+open X64.Vale.Lemmas_i
+module TS = X64.Taint_Semantics_s
+module ME = X64.Memory_i_s
+module BS = X64.Bytes_Semantics_s
 #set-options "--z3rlimit 40"
 
 open Vale_memcpy
@@ -154,9 +159,21 @@ let lin_implies_post (va_s0:va_state) (va_sM:va_state) (va_fM:va_fuel) (dst:s8) 
   length_t_eq (TBase TUInt64) src;
   ()
 
-val lin_ghost_memcpy: dst:s8 -> src:s8 ->  stack_b:b8 -> (h0:HS.mem{pre_cond h0 dst src /\ B.length stack_b == 24 /\ live h0 stack_b /\ buf_disjoint_from stack_b [dst;src]}) -> GTot (h1:HS.mem{post_cond h0 h1 dst src })
+let lin_calling_conv (s0:TS.traceState) (s1:TS.traceState) =
+  let s0_b= s0.TS.state.ME.state in
+  let s_b = s1.TS.state.ME.state in
+  // Ensures that the execution didn't crash
+  s_b.BS.ok /\
+  // Ensures that the callee_saved registers are correct
+  s0_b.BS.regs Rbx == s_b.BS.regs Rbx /\
+  s0_b.BS.regs Rbp == s_b.BS.regs Rbp /\
+  s0_b.BS.regs R12 == s_b.BS.regs R12 /\
+  s0_b.BS.regs R13 == s_b.BS.regs R13 /\
+  s0_b.BS.regs R14 == s_b.BS.regs R14 /\
+  s0_b.BS.regs R15 == s_b.BS.regs R15
 
-let lin_ghost_memcpy dst src stack_b h0 =
+
+let create_initial_state dst src stack_b (h0:HS.mem{pre_cond h0 dst src /\ B.length stack_b == 24 /\ live h0 stack_b /\ buf_disjoint_from stack_b [dst;src]}) : GTot TS.traceState =
   let taint_func (x:b8) : GTot taint =
     if StrongExcludedMiddle.strong_excluded_middle (x == dst) then Secret else
     if StrongExcludedMiddle.strong_excluded_middle (x == src) then Secret else
@@ -172,29 +189,50 @@ let lin_ghost_memcpy dst src stack_b h0 =
     | Rsi -> addr_src
     | _ -> init_regs r end in
   let xmms = init_xmms in
-  let s0 = {ok = true; regs = regs; xmms = xmms; flags = 0; mem = mem; memTaint = create_valid_memtaint mem buffers taint_func} in
+  let (s_b:BS.state) = {BS.ok = true; BS.regs = regs; BS.xmms = xmms; BS.flags = 0; BS.mem = Interop.down_mem mem.hs mem.addrs mem.ptrs} in
+  let s0:X64.Memory_i_s.state = {ME.state = s_b; ME.mem = mem} in
+  {TS.state = s0; TS.trace = []; TS.memTaint = create_valid_memtaint mem buffers taint_func}
+
+val lin_ghost_memcpy: dst:s8 -> src:s8 ->  stack_b:b8 -> (h0:HS.mem{pre_cond h0 dst src /\ B.length stack_b == 24 /\ live h0 stack_b /\ buf_disjoint_from stack_b [dst;src]}) -> GTot 
+  (s1:TS.traceState{post_cond h0 (s1.TS.state.ME.mem.hs) dst src /\ lin_calling_conv (create_initial_state dst src stack_b h0) s1})
+//(h1:HS.mem{post_cond h0 h1 dst src })
+
+val lemma_lin_ghost_memcpy:  dst:s8 -> src:s8 ->  stack_b:b8 -> (h0:HS.mem{pre_cond h0 dst src /\ B.length stack_b == 24 /\ live h0 stack_b /\ buf_disjoint_from stack_b [dst;src]}) ->
+  Ghost nat
+    (requires True)
+    (ensures (fun f1 ->
+      (let s0 = create_initial_state dst src stack_b h0 in
+       let s1 = TS.taint_eval_code (va_code_memcpy false) f1 s0 in
+       Some? s1 /\
+       post_cond h0 ((Some?.v s1).TS.state.ME.mem.hs) dst src /\
+       lin_calling_conv s0 (Some?.v s1))
+      )
+    )
+
+let lemma_lin_ghost_memcpy dst src stack_b h0 =
   length_t_eq (TBase TUInt64) stack_b;
   length_t_eq (TBase TUInt64) dst;
   length_t_eq (TBase TUInt64) src;
   lin_implies_pre h0 dst src stack_b ;
-  let s1, f1 = va_lemma_memcpy (va_code_memcpy false) s0 false stack_b dst src  in
-  // Ensures that the Vale execution was correct
-  assert(s1.ok);
-  // Ensures that the callee_saved registers are correct
-  assert(s0.regs Rbx == s1.regs Rbx);
-  assert(s0.regs Rbp == s1.regs Rbp);
-  assert(s0.regs R12 == s1.regs R12);
-  assert(s0.regs R13 == s1.regs R13);
-  assert(s0.regs R14 == s1.regs R14);
-  assert(s0.regs R15 == s1.regs R15);
-  // Ensures that va_code_memcpy is actually Vale code, and that s1 is the result of executing this code
-  assert (va_ensure_total (va_code_memcpy false) s0 s1 f1);
-  lin_implies_post s0 s1 f1 dst src stack_b ;
-  s1.mem.hs
+  let s0 = create_initial_state dst src stack_b h0 in
+  let s_v, f_v = va_lemma_memcpy (va_code_memcpy false) (state_of_S s0) false stack_b dst src in  
+  lin_implies_post (state_of_S s0) s_v f_v dst src stack_b;
+  f_v
+  
+
+let lin_ghost_memcpy dst src stack_b h0 =
+  let s0 = create_initial_state dst src stack_b h0 in
+
+  let f1 = lemma_lin_ghost_memcpy dst src stack_b h0 in
+  let s1 = TS.taint_eval_code (va_code_memcpy false) f1 s0 in
+  (Some?.v s1)
+
+val ghost_memcpy: dst:s8 -> src:s8 ->  stack_b:b8 -> (h0:HS.mem{pre_cond h0 dst src /\ B.length stack_b == 24 /\ live h0 stack_b /\ buf_disjoint_from stack_b [dst;src]}) -> GTot 
+  (h1:HS.mem{post_cond h0 h1 dst src})
 
 let ghost_memcpy dst src stack_b h0 =
   if win then win_ghost_memcpy dst src stack_b h0
-  else lin_ghost_memcpy dst src stack_b h0
+  else (lin_ghost_memcpy dst src stack_b h0).TS.state.ME.mem.hs
 
 let memcpy dst src  =
   push_frame();
